security exploration

PathORAMcoq/Security.v
@@ -1,6 +1,6 @@
 Require Import FCF.FCF.
 
-Definition  bool_eq_dec : eq_dec bool.
+Definition bool_eq_dec : eq_dec bool.
 Proof.
   unfold eq_dec.
   decide equality.
@@ -11,7 +11,16 @@ Definition coin_flip : Comp bool.
   exact (Bind rnd_bv (fun bv => Ret bool_eq_dec (Vector.hd bv))).
 Defined.
 
+Compute evalDist coin_flip true.
+Print Rat.
+Print posnat.
+Print sig.
+Definition Rat_to_nums (r : Rat) : nat * nat :=
+  match r with
+  | RatIntro numerator (exist _ denominator _) => (numerator, denominator)
+  end.
 
+Compute Rat_to_nums (evalDist coin_flip false).
 
 (* uniform distribution.  *)
 
@@ -19,15 +28,62 @@ Definition uniform_comp(l : nat): Comp (Bvector l) := Rnd l.
 
 Definition uniform_dist (l : nat) := evalDist (uniform_comp l).
 
-Definition sampleBV := Vector.cons _ false _ (Vector.cons _ true _ (Vector.nil _)).
-Compute uniform_dist 2 sampleBV.
-Definition sampleBV' := Vector.cons _ true _ (Vector.nil _).
-Compute uniform_dist 1 sampleBV'.
+Definition sampleBV1 := Vector.cons _ false _ (Vector.cons _ true _ (Vector.nil _)).
+Compute uniform_dist 2 sampleBV1.
+
+Definition sampleBV2 := Vector.cons _ false _ (Vector.cons _ true _ (Vector.nil _)).
+Compute uniform_dist 2 sampleBV2.
+
+#[export] Instance bool_eqb : EqDec bool :=
+  {
+    eqb := Bool.eqb;
+    eqb_leibniz := eqb_true_iff
+  }.
+Lemma Bv12Equiv : eqb_vector bool_eqb sampleBV1 sampleBV2 = true.
+Proof.
+  unfold eqb_vector.
+  simpl.
+  reflexivity.
+Qed.
+
+(* assume that the tree has one node and 2 leaves, then the path is 1 bit long *)
+(**
+                 / [ ID | PAYLOAD ] \
+                 | [ ID | PAYLOAD ] |
+                 \ [ ID | PAYLOAD ] /
+                  /               \
+                 /                 \
+                /                   \
+   / [ ID | PAYLOAD ] \   / [ ID | PAYLOAD ] \  ←
+   | [ ID | PAYLOAD ] |   | [ ID | PAYLOAD ] |  ← A BUCKET = N BLOCKS (example: N=3)
+   \ [ ID | PAYLOAD ] /   \ [ ID | PAYLOAD ] /  ←
+                            ↑↑↑↑↑↑↑↑↑↑↑↑↑↑↑↑
+ **)
+
+(*
+  Z = 3
+  N = 3
+  addr space = Z * N = 3 * 3
+  path_len = 1 bit 
+  |acc_list| = Len = 5
+  Len_AP = 1 * 5 = 5 bits
+ *)
+
+(*TODO : define 2 random variables from a coin_flip, show that the probability of the conjuction of them is true is 1/4 *)
+(*
+  p <- coin_flip
+  q <- coin_flip
+  Pr[p /\ q ] = 1/4
+ *)
 
 
-(* conditional probability *)
 
 
 
 
- 
+
+
+
+
+
+
